thys/MFODL_Monitor_Devel/Monitor_Impl.thy
@@ -33,15 +33,6 @@ derive (rbt) mapping_impl string8
 derive (rbt) set_impl event_data
 derive (rbt) mapping_impl event_data
 
-definition add_new_mmuaux' :: "args \<Rightarrow> event_data table \<Rightarrow> event_data table \<Rightarrow> ts \<Rightarrow> event_data mmuaux \<Rightarrow>
-  event_data mmuaux" where
-  "add_new_mmuaux' = add_new_mmuaux"
-
-interpretation muaux valid_mmuaux init_mmuaux add_new_mmuaux' length_mmuaux eval_mmuaux
-  using valid_init_mmuaux valid_add_new_mmuaux valid_length_mmuaux valid_eval_mmuaux
-  unfolding add_new_mmuaux'_def
-  by unfold_locales assumption+
-
 type_synonym 'a vmsaux = "nat \<times> (nat \<times> 'a table) list"
 
 definition valid_vmsaux :: "args \<Rightarrow> nat \<Rightarrow> event_data vmsaux \<Rightarrow>
@@ -66,8 +57,8 @@ definition add_new_table_vmsaux :: "args \<Rightarrow> event_data table \<Righta
   | ((t, y) # ts) \<Rightarrow> if t = cur then (t, y \<union> rel2) # ts else (cur, rel2) # auxlist)))"
 
 definition result_vmsaux :: "args \<Rightarrow> event_data vmsaux \<Rightarrow> event_data table" where
-  "result_vmsaux = (\<lambda>args (cur, auxlist).
-    foldr (\<union>) [rel. (t, rel) \<leftarrow> auxlist, memL (args_ivl args) (cur - t)] {})"
+  "result_vmsaux = (\<lambda>args (cur, auxlist). eval_args_agg args
+    (foldr (\<union>) [rel. (t, rel) \<leftarrow> auxlist, memL (args_ivl args) (cur - t)] {}))"
 
 type_synonym 'a vmuaux = "nat \<times> (nat \<times> 'a table \<times> 'a table) list"
 
@@ -88,13 +79,15 @@ definition length_vmuaux :: "args \<Rightarrow> event_data vmuaux \<Rightarrow> 
 definition eval_vmuaux :: "args \<Rightarrow> nat \<Rightarrow> event_data vmuaux \<Rightarrow>
   event_data table list \<times> event_data vmuaux" where
   "eval_vmuaux = (\<lambda>args nt (t, auxlist).
-    (let (res, auxlist') = eval_until (args_ivl args) nt auxlist in (res, (t, auxlist'))))"
+    (let (res, auxlist') = eval_until (args_ivl args) nt auxlist in (map (eval_args_agg args) res, (t, auxlist'))))"
 
 global_interpretation verimon_maux: maux valid_vmsaux init_vmsaux add_new_ts_vmsaux join_vmsaux
   add_new_table_vmsaux result_vmsaux valid_vmuaux init_vmuaux add_new_vmuaux length_vmuaux
   eval_vmuaux
   defines vminit0 = "maux.minit0 (init_vmsaux :: _ \<Rightarrow> event_data vmsaux) (init_vmuaux :: _ \<Rightarrow> event_data vmuaux) :: _ \<Rightarrow> Formula.formula \<Rightarrow> _"
   and vminit = "maux.minit (init_vmsaux :: _ \<Rightarrow> event_data vmsaux) (init_vmuaux :: _ \<Rightarrow> event_data vmuaux) :: Formula.formula \<Rightarrow> _"
+  and vminit_since = "verimon_maux.init_since"
+  and vminit_until = "verimon_maux.init_until"
   and vminit_safe = "maux.minit_safe (init_vmsaux :: _ \<Rightarrow> event_data vmsaux) (init_vmuaux :: _ \<Rightarrow> event_data vmuaux) :: Formula.formula \<Rightarrow> _"
   and vmupdate_since = "maux.update_since add_new_ts_vmsaux join_vmsaux add_new_table_vmsaux (result_vmsaux :: _ \<Rightarrow> event_data vmsaux \<Rightarrow> event_data table)"
   and vmeval = "maux.meval add_new_ts_vmsaux join_vmsaux add_new_table_vmsaux (result_vmsaux :: _ \<Rightarrow> event_data vmsaux \<Rightarrow> _) add_new_vmuaux (eval_vmuaux :: _ \<Rightarrow> _ \<Rightarrow> event_data vmuaux \<Rightarrow> _)"
@@ -107,17 +100,19 @@ global_interpretation verimon_maux: maux valid_vmsaux init_vmsaux add_new_ts_vms
     length_vmuaux_def eval_vmuaux_def
   by unfold_locales auto
 
-global_interpretation default_maux: maux valid_mmsaux "init_mmsaux :: _ \<Rightarrow> event_data mmsaux" add_new_ts_mmsaux gc_join_mmsaux add_new_table_mmsaux result_mmsaux
-  valid_mmuaux "init_mmuaux :: _ \<Rightarrow> event_data mmuaux" add_new_mmuaux' length_mmuaux eval_mmuaux
+global_interpretation default_maux: maux valid_mmsaux "init_mmsaux :: _ \<Rightarrow> event_data mmsaux" add_new_ts_mmsaux gc_join_mmsaux add_new_table_mmsaux result_mmsaux'
+  valid_mmuaux "init_mmuaux :: _ \<Rightarrow> event_data mmuaux" add_new_mmuaux length_mmuaux eval_mmuaux'
   defines minit0 = "maux.minit0 (init_mmsaux :: _ \<Rightarrow> event_data mmsaux) (init_mmuaux :: _ \<Rightarrow> event_data mmuaux) :: _ \<Rightarrow> Formula.formula \<Rightarrow> _"
   and minit = "maux.minit (init_mmsaux :: _ \<Rightarrow> event_data mmsaux) (init_mmuaux :: _ \<Rightarrow> event_data mmuaux) :: Formula.formula \<Rightarrow> _"
+  and minit_since = "default_maux.init_since"
+  and minit_until = "default_maux.init_until"
   and minit_safe = "maux.minit_safe (init_mmsaux :: _ \<Rightarrow> event_data mmsaux) (init_mmuaux :: _ \<Rightarrow> event_data mmuaux) :: Formula.formula \<Rightarrow> _"
-  and mupdate_since = "maux.update_since add_new_ts_mmsaux gc_join_mmsaux add_new_table_mmsaux (result_mmsaux :: _ \<Rightarrow> event_data mmsaux \<Rightarrow> event_data table)"
-  and meval = "maux.meval add_new_ts_mmsaux gc_join_mmsaux add_new_table_mmsaux (result_mmsaux :: _ \<Rightarrow> event_data mmsaux \<Rightarrow> _) add_new_mmuaux' (eval_mmuaux :: _ \<Rightarrow> _ \<Rightarrow> event_data mmuaux \<Rightarrow> _)"
-  and mstep = "maux.mstep add_new_ts_mmsaux gc_join_mmsaux add_new_table_mmsaux (result_mmsaux :: _ \<Rightarrow> event_data mmsaux \<Rightarrow> _) add_new_mmuaux' (eval_mmuaux :: _ \<Rightarrow> _ \<Rightarrow> event_data mmuaux \<Rightarrow> _)"
-  and msteps0_stateless = "maux.msteps0_stateless add_new_ts_mmsaux gc_join_mmsaux add_new_table_mmsaux (result_mmsaux :: _ \<Rightarrow> event_data mmsaux \<Rightarrow> _) add_new_mmuaux' (eval_mmuaux :: _ \<Rightarrow> _ \<Rightarrow> event_data mmuaux \<Rightarrow> _)"
-  and msteps_stateless = "maux.msteps_stateless add_new_ts_mmsaux gc_join_mmsaux add_new_table_mmsaux (result_mmsaux :: _ \<Rightarrow> event_data mmsaux \<Rightarrow> _) add_new_mmuaux' (eval_mmuaux :: _ \<Rightarrow> _ \<Rightarrow> event_data mmuaux \<Rightarrow> _)"
-  and monitor = "maux.monitor init_mmsaux add_new_ts_mmsaux gc_join_mmsaux add_new_table_mmsaux (result_mmsaux :: _ \<Rightarrow> event_data mmsaux \<Rightarrow> _) init_mmuaux add_new_mmuaux' (eval_mmuaux :: _ \<Rightarrow> _ \<Rightarrow> event_data mmuaux \<Rightarrow> _)"
+  and mupdate_since = "maux.update_since add_new_ts_mmsaux gc_join_mmsaux add_new_table_mmsaux result_mmsaux'"
+  and meval = "maux.meval add_new_ts_mmsaux gc_join_mmsaux add_new_table_mmsaux result_mmsaux' add_new_mmuaux eval_mmuaux'"
+  and mstep = "maux.mstep add_new_ts_mmsaux gc_join_mmsaux add_new_table_mmsaux result_mmsaux' add_new_mmuaux eval_mmuaux'"
+  and msteps0_stateless = "maux.msteps0_stateless add_new_ts_mmsaux gc_join_mmsaux add_new_table_mmsaux result_mmsaux' add_new_mmuaux eval_mmuaux'"
+  and msteps_stateless = "maux.msteps_stateless add_new_ts_mmsaux gc_join_mmsaux add_new_table_mmsaux result_mmsaux' add_new_mmuaux eval_mmuaux'"
+  and monitor = "maux.monitor init_mmsaux add_new_ts_mmsaux gc_join_mmsaux add_new_table_mmsaux result_mmsaux' init_mmuaux add_new_mmuaux eval_mmuaux'"
   by unfold_locales
 
 lemma image_these: "f ` Option.these X = Option.these (map_option f ` X)"
@@ -326,8 +321,8 @@ lemma upd_nested_max_tstp_code[code]:
     else Code.abort (STR ''upd_nested_max_tstp: infinite'') (\<lambda>_. upd_nested_max_tstp m d X))"
   by transfer (auto simp add: upd_nested_max_tstp_fold)
 
-declare [[code drop: add_new_mmuaux']]
-declare add_new_mmuaux'_def[unfolded add_new_mmuaux.simps, folded upd_nested_max_tstp_def, code]
+declare [[code drop: add_new_mmuaux]]
+declare add_new_mmuaux.simps[folded upd_nested_max_tstp_def, code]
 
 lemma filter_set_empty[simp]: "filter_set m {} t = m"
   unfolding filter_set_def
